More progress in resuming solver.

PropositionalLogic/DeepEmbedded/Deep.v
@@ -4,6 +4,7 @@ Require Import Logic.MinimumLogic.ProofTheory.Minimum.
 Require Import Logic.PropositionalLogic.Syntax.
 Require Import Logic.PropositionalLogic.ProofTheory.Intuitionistic.
 Require Import Logic.PropositionalLogic.ProofTheory.TheoryOfIteratedConnectives.
+Require Import Logic.PropositionalLogic.ProofTheory.TheoryOfPropositionalConnectives.
 
 Local Open Scope logic_base.
 Local Open Scope syntax.
@@ -14,6 +15,9 @@ Inductive expr : Type :=
 | impp : expr -> expr -> expr
 | varp : nat -> expr
 .
+
+Definition truep: expr := impp (varp 0) (varp 0).
+Definition iffp x y: expr := andp (impp x y) (impp y x).
 
 Fixpoint beq e1 e2 :=
   match e1, e2 with
@@ -42,6 +46,15 @@ Local Instance minL : MinimumLanguage L := Build_MinimumLanguage L impp.
 Local Instance andpL : AndLanguage L :=
   Build_AndLanguage L andp.
 
+Local Instance truepL : TrueLanguage L :=
+  Build_TrueLanguage L truep.
+
+Local Instance iffpL : IffLanguage L :=
+  Build_IffLanguage L iffp.
+
+Local Instance iffpDef : IffDefinition_And_Imp L :=
+  AndImp2Iff_Normal.
+
 Local Instance iter_andp_L: IterAndLanguage L :=
   Build_IterAndLanguage L (fun es => fold_left andp es truep).
 
@@ -64,13 +77,25 @@ Proof.
   + apply axiom2.
 Qed.
 
-Local Instance andpAX: AndpAxiomatization L GP.
+Local Instance andpAX: AndAxiomatization L GP.
 Proof.
   constructor.
   + apply andp_intros.
   + apply andp_elim1.
   + apply andp_elim2.
 Qed.
+
+Local Instance truepAX: TrueAxiomatization L GP.
+Proof.
+  constructor.
+  simpl.
+  unfold truep.
+  pose proof provable_impp_refl (varp 0).
+  exact H.
+Qed.
+
+Local Instance iffpAX: IffAxiomatization L GP :=
+  IffFromDefToAX_And_Imp.
 
 Local Instance iter_andp_DL: IterAndDefinition_left L :=
   Build_IterAndDefinition_left L _ _ _ (fun es => eq_refl).
